matching-logic/src/FixpointReasoning.v
@@ -733,7 +733,7 @@ Section with_signature.
             simpl in mp.
             epose proof (Htot := (list_lookup_lookup_total_lt (rev (d0 :: x' :: l')) 1 _)).
             Unshelve. 2: { constructor. exact d0. }
-            2: { simpl. rewrite app_length. rewrite app_length. simpl.  lia.  }
+            2: { simpl. rewrite length_app. rewrite length_app. simpl.  lia.  }
 
             remember (@lookup_total nat (@Domain Σ M) (list (@Domain Σ M))
                  (@list_lookup_total (@Domain Σ M) {| inhabitant := d0 |}) (S O)
@@ -786,7 +786,7 @@ Section with_signature.
               inversion H2. subst x' l'. clear H2.
               simpl in Htot.
               destruct (l ++ [m]) eqn:Hcontra.
-              { pose proof (Hcontra' := @app_length _ l [m]).
+              { pose proof (Hcontra' := @length_app _ l [m]).
                 rewrite Hcontra in Hcontra'.
                 simpl in Hcontra'. lia.
               }
