matching-logic/src/Theories/Bool_Semantics.v
@@ -1,22 +1,9 @@
-From Coq Require Import ssreflect ssrfun ssrbool.
-
-Require Import Setoid.
-From Coq Require Import Unicode.Utf8.
-From Coq.Logic Require Import Classical_Prop FunctionalExtensionality.
-From Coq.Classes Require Import Morphisms_Prop.
-
-From stdpp Require Import base sets.
-
-From MatchingLogic Require Export
-    Logic
-    Utils.extralibrary
-    Theories.Bool_Syntax
-    Theories.ModelExtension.
-
-Import MatchingLogic.Theories.Definedness_Syntax.Notations.
-Import MatchingLogic.Theories.Bool_Syntax.Notations.
-Import BoundVarSugar.
-Import MatchingLogic.Semantics.Notations.
+From Coq Require Import Classes.Morphisms_Prop.
+From MatchingLogic Require Export Sorts_Semantics
+                                  Bool_Syntax.
+Import MatchingLogic.Logic.Notations
+       MatchingLogic.Theories.Definedness_Syntax.Notations
+       MatchingLogic.Theories.Sorts_Syntax.Notations.
 
 Section with_model.
   Context
